messageInvariantPrototypes/paxos/decentralizedMonotonic/messageInvariants.dfy
@@ -1,0 +1,358 @@
+include "spec.dfy"
+
+module PaxosMessageInvariants {
+
+import opened Types
+import opened UtilitiesLibrary
+import opened DistributedSystem
+import opened Obligations
+
+// certified self-inductive
+// Every message in the network has a valid source
+ghost predicate ValidMessageSrc(c: Constants, v: Variables) 
+  requires v.WF(c)
+{
+  forall msg | msg in v.network.sentMsgs 
+  :: 
+  match msg 
+    case Prepare(bal) => c.ValidLeaderIdx(bal)
+    case Promise(_, acc, _) => c.ValidAcceptorIdx(acc)
+    case Propose(bal, _) => c.ValidLeaderIdx(bal)
+    case Accept(_, acc) => c.ValidAcceptorIdx(acc)
+    case Learn(lnr, _, _) => c.ValidLearnerIdx(lnr)
+}
+
+// Message bundle
+ghost predicate MessageInv(c: Constants, v: Variables) 
+{
+  && v.WF(c)
+  && ValidMessageSrc(c, v)
+  // From Leader transitions
+  // && LeaderValidReceivedPromises(c, v)
+  && ValidProposeMesssage(c, v)
+  // // From Acceptor transitions
+  && AcceptorValidAccepted(c, v)
+  && ValidPromiseMessage(c, v)
+  // && ValidAcceptMessage(c, v)
+  // // From Learner transitions
+  // && LearnerValidReceivedAccepts(c, v)
+  // && ValidLearnMessage(c, v)
+}
+
+lemma InitImpliesMessageInv(c: Constants, v: Variables)
+  requires Init(c, v)
+  ensures MessageInv(c, v)
+{
+}
+
+lemma MessageInvInductive(c: Constants, v: Variables, v': Variables)
+  requires MessageInv(c, v)
+  requires Next(c, v, v')
+  ensures MessageInv(c, v')
+{
+  // InvNextLeaderValidReceivedPromises(c, v, v');
+  InvNextValidProposeMesssage(c, v, v');
+  InvNextValidPromiseMessage(c, v, v');
+  // InvNextValidAcceptMessage(c, v, v');
+}
+
+/***************************************************************************************
+*                                     Leader Host                                      *
+***************************************************************************************/
+
+// certified self-inductive
+// Leader updates receivedPromises based on Promise messages
+// Property of Receive
+// ghost predicate LeaderValidReceivedPromises(c: Constants, v: Variables)
+//   requires v.WF(c)
+// {
+//   forall idx, i, p | 
+//     && c.ValidLeaderIdx(idx)
+//     && 0 <= i < |v.leaders[idx].receivedPromises|
+//     && p in v.leaders[idx].receivedPromises[i]
+//   :: 
+//     IsPromiseMessage(v, p)
+// }
+
+// certified self-inductive
+// Property of Send
+ghost predicate ValidProposeMesssage(c: Constants, v: Variables)
+  requires v.WF(c)
+  requires ValidMessageSrc(c, v)
+{
+  forall prop | IsProposeMessage(v, prop)
+  ::
+    (exists i ::
+      && 0 <= i < |v.leaders[prop.bal].h|
+      && var vi := v.leaders[prop.bal].h[i];
+      && vi.CanPropose(c.leaderConstants[prop.bal])
+      && prop.val == vi.value
+    )
+}
+
+/***************************************************************************************
+*                                     Acceptor Host                                    *
+***************************************************************************************/
+
+// certified self-inductive
+// Acceptor updates its acceptedVB based on a Propose message carrying that ballot 
+// and value
+ghost predicate AcceptorValidAccepted(c: Constants, v: Variables)
+  requires v.WF(c)
+{
+  forall idx, i |
+    && c.ValidAcceptorIdx(idx) 
+    && 0 <= i < |v.acceptors[idx].h|
+    && v.acceptors[idx].h[i].acceptedVB.Some?
+  :: 
+    && var vb :=v.acceptors[idx].h[i].acceptedVB.value;
+    && Propose(vb.b, vb.v) in v.network.sentMsgs
+}
+
+// certified self-inductive
+// Every Promise message ballot reflects acceptor's local promised history, and 
+// it's vbOpt represents a prior accepted value
+// Property of Send
+ghost predicate ValidPromiseMessage(c: Constants, v: Variables) 
+  requires v.WF(c)
+  requires ValidMessageSrc(c, v)
+{
+  forall prom | IsPromiseMessage(v, prom)
+  ::
+  (exists i :: PromiseMessageMatchesHistory(c, v, prom, i))
+}
+
+ghost predicate PromiseMessageMatchesHistory(c: Constants, v: Variables, prom: Message, i: nat)
+  requires v.WF(c)
+  requires ValidMessageSrc(c, v)
+  requires IsPromiseMessage(v, prom)
+{
+  && 0 <= i < |v.acceptors[prom.acc].h|
+  && v.acceptors[prom.acc].h[i].promised.Some?
+  && prom.bal == v.acceptors[prom.acc].h[i].promised.value
+  && prom.vbOpt == v.acceptors[prom.acc].h[i].acceptedVB
+}
+
+// // certified self-inductive
+// // Every Accept message reflects acceptor state history
+// // Property of Send
+// ghost predicate ValidAcceptMessage(c: Constants, v: Variables)
+//   requires v.WF(c)
+//   requires ValidMessageSrc(c, v)
+// {
+//   forall accept | IsAcceptMessage(v, accept)
+//   ::
+//   (exists i :: 
+//     && 0 <= i < |v.acceptors[accept.acc].acceptedVB|
+//     && v.acceptors[accept.acc].acceptedVB[i] == Some(accept.vb)
+//     && v.acceptors[accept.acc].promised[i] == accept.vb.b
+//   )
+// }
+
+
+/***************************************************************************************
+*                                     Learner Host                                     *
+***************************************************************************************/
+
+// // certified self-inductive
+// // Learner updates its receivedAccepts map based on a Accept message carrying that 
+// // accepted ValBal pair
+// // Property of Receive
+// ghost predicate LearnerValidReceivedAccepts(c: Constants, v: Variables) 
+//   requires v.WF(c)
+// {
+//   forall idx, vb, acc, i | 
+//     && c.ValidLearnerIdx(idx)
+//     && vb in v.learners[idx].receivedAccepts
+//     && 0 <= i < |v.learners[idx].receivedAccepts[vb]|
+//     && acc in v.learners[idx].receivedAccepts[vb][i]
+//   ::
+//     Accept(vb, acc) in v.network.sentMsgs
+// }
+
+// // certified self-inductive
+// ghost predicate ValidLearnMessage(c: Constants, v: Variables)
+//   requires v.WF(c)
+//   requires ValidMessageSrc(c, v)
+// {
+//   forall learn | IsLearnMessage(v, learn)
+//   :: 
+//   VB(learn.val, learn.bal) in v.learners[learn.lnr].learned
+// }
+
+
+/***************************************************************************************
+*                               Proofs (how unfortunate)                               *
+***************************************************************************************/
+
+
+// lemma InvNextLeaderValidReceivedPromises(c: Constants, v: Variables, v': Variables)
+//   requires v.WF(c)
+//   requires LeaderValidReceivedPromises(c, v)
+//   requires Next(c, v, v')
+//   ensures LeaderValidReceivedPromises(c, v')
+// {
+//   forall idx, i, p | 
+//     && c.ValidLeaderIdx(idx)
+//     && 0 <= i < |v'.leaders[idx].receivedPromises|
+//     && p in v'.leaders[idx].receivedPromises[i]
+//   ensures
+//     IsPromiseMessage(v', p)
+//   {
+//     assert IsPromiseMessage(v, p);  // trigger
+//   }
+// }
+
+
+// Tony: This message invariant requires proof. What do I make of this?
+// Because dafny can't handle alternating quantifiers
+lemma InvNextValidProposeMesssage(c: Constants, v: Variables, v': Variables)
+  requires v.WF(c)
+  requires ValidMessageSrc(c, v)
+  requires ValidProposeMesssage(c, v)
+  requires Next(c, v, v')
+  ensures ValidProposeMesssage(c, v')
+{
+  forall prop | IsProposeMessage(v', prop)
+  ensures
+    (exists i ::
+      && 0 <= i < |v'.leaders[prop.bal].h|
+      && var vi := v'.leaders[prop.bal].h[i];
+      && vi.CanPropose(c.leaderConstants[prop.bal])
+      && prop.val == vi.value
+    )
+  {
+    var dsStep :| NextStep(c, v, v', dsStep);
+    var actor, msgOps := dsStep.actor, dsStep.msgOps;
+    var i: int;
+    if dsStep.LeaderStep? && actor == prop.bal {
+      if msgOps.send == Some(prop) {
+        // witness
+        i := |v.leaders[prop.bal].h| - 1;
+      } else {
+        assert IsProposeMessage(v, prop);
+        // witness
+        i :|       
+            && 0 <= i < |v.leaders[prop.bal].h|
+            && var vi := v.leaders[prop.bal].h[i];
+            && vi.CanPropose(c.leaderConstants[prop.bal])
+            && prop.val == vi.value;
+      }
+      // trigger
+      assert  
+        && 0 <= i < |v'.leaders[prop.bal].h|
+        && var vi := v'.leaders[prop.bal].h[i];
+        && vi.CanPropose(c.leaderConstants[prop.bal])
+        && prop.val == vi.value;
+    }
+  }
+}
+
+// Because dafny can't handle alternating quantifiers
+lemma InvNextValidPromiseMessage(c: Constants, v: Variables, v': Variables)
+  requires v.WF(c)
+  requires ValidMessageSrc(c, v)
+  requires ValidPromiseMessage(c, v)
+  requires Next(c, v, v')
+  ensures ValidPromiseMessage(c, v')
+{
+  forall prom | IsPromiseMessage(v', prom)
+  ensures
+    exists i :: PromiseMessageMatchesHistory(c, v', prom, i)
+  {
+    var dsStep :| NextStep(c, v, v', dsStep);
+    var actor, msgOps := dsStep.actor, dsStep.msgOps;
+    if && dsStep.AcceptorStep? 
+       && prom.acc == actor 
+       && msgOps.send == Some(prom)
+    {
+      var ac, a, a' := c.acceptorConstants[actor], v.acceptors[actor], v'.acceptors[actor];
+      var step :| AcceptorHost.NextStep(ac, a, a', step, msgOps);
+      if step.MaybePromiseStep? {
+        var doPromise := a.Last().promised.None? || (a.Last().promised.Some? && a.Last().promised.value < a.Last().pendingPrepare.value.bal);
+        if doPromise {
+          assert PromiseMessageMatchesHistory(c, v', prom, |a'.h|-1);  // trigger
+        }
+      }
+      assume false;
+    } else {
+      assert IsPromiseMessage(v, prom);  // trigger
+      var i :| PromiseMessageMatchesHistory(c, v, prom, i);  // witness
+      assert PromiseMessageMatchesHistory(c, v', prom, i);   // trigger
+    }
+  }
+}
+
+// // Because dafny can't handle alternating quantifiers
+// lemma InvNextValidAcceptMessage(c: Constants, v: Variables, v': Variables)
+//   requires v.WF(c)
+//   requires ValidMessageSrc(c, v)
+//   requires ValidAcceptMessage(c, v)
+//   requires Next(c, v, v')
+//   ensures ValidAcceptMessage(c, v')
+// {
+//   forall accept | IsAcceptMessage(v', accept)
+//   ensures exists i :: 
+//     && 0 <= i < |v'.acceptors[accept.acc].acceptedVB|
+//     && v'.acceptors[accept.acc].acceptedVB[i] == Some(accept.vb)
+//     && v'.acceptors[accept.acc].promised[i] == accept.vb.b
+//   {
+//     var dsStep :| NextStep(c, v, v', dsStep);
+//     var actor, msgOps := dsStep.actor, dsStep.msgOps;
+//     if && dsStep.AcceptorStep? 
+//        && accept.acc == actor 
+//        && msgOps.send == Some(accept)
+//     {
+//       var ac, a, a' := c.acceptorConstants[actor], v.acceptors[actor], v'.acceptors[actor];
+//       var step :| AcceptorHost.NextStep(ac, a, a', step, msgOps);
+//       if step.ReceiveStep? && msgOps.recv.value.Propose? {
+//         var doAccept := a.PromisedNone() || a.GetPromised() <= msgOps.recv.value.bal;
+//         if doAccept {
+//           var i := |a'.acceptedVB|-1;
+//           assert v'.acceptors[accept.acc].acceptedVB[i] == Some(accept.vb); // trigger
+//           assert v'.acceptors[accept.acc].promised[i] == accept.vb.b;       // trigger
+//         }
+//       }
+//     } else {
+//       assert IsAcceptMessage(v, accept);  // trigger
+//       var i :|  && 0 <= i < |v.acceptors[accept.acc].acceptedVB|   // witness
+//                 && v.acceptors[accept.acc].acceptedVB[i] == Some(accept.vb)
+//                 && v.acceptors[accept.acc].promised[i] == accept.vb.b;
+//       assert  && 0 <= i < |v'.acceptors[accept.acc].acceptedVB|    // trigger
+//               && v'.acceptors[accept.acc].acceptedVB[i] == Some(accept.vb)
+//               && v'.acceptors[accept.acc].promised[i] == accept.vb.b;
+//     }
+//   }
+// }
+
+
+/***************************************************************************************
+*                                        Utils                                         *
+***************************************************************************************/
+
+ghost predicate IsPrepareMessage(v: Variables, m: Message) {
+  && m.Prepare?
+  && m in v.network.sentMsgs
+}
+
+ghost predicate IsPromiseMessage(v: Variables, m: Message) {
+  && m.Promise?
+  && m in v.network.sentMsgs
+}
+
+ghost predicate IsProposeMessage(v: Variables, m: Message) {
+  && m.Propose?
+  && m in v.network.sentMsgs
+}
+
+ghost predicate IsAcceptMessage(v: Variables, m: Message) {
+  && m.Accept?
+  && m in v.network.sentMsgs
+}
+
+ghost predicate IsLearnMessage(v: Variables, m: Message) {
+  && m.Learn?
+  && m in v.network.sentMsgs
+} 
+}  // end module PaxosProof
+
